Replace nats by integers: renamings
tnat -> tint
TNat -> TInt
vnat -> vint
lnat -> lint
bin_op_eval_nat -> bin_op_eval_int
oNat -> oInt
𝐍 -> 𝐙

scala-examples/coqTranslation/scalaLibV.scala
@@ -6,7 +6,7 @@ import typing_unstamped_derivedV._
 type Nat = Int // Hack
 
 type HashableString = { val hashCode_ : () => Nat }
-// Notation HashableString := (μ {@ val "hashCode" : TUnit →: TNat }).
+// Notation HashableString := (μ {@ val "hashCode" : TUnit →: TInt }).
 
 object loopDefV { self =>
   val loop : Any => Nothing = v => self.loop(v)
