theories/Dot/examples/examples.v
@@ -28,7 +28,7 @@ Proof. have ? := loopDefTyp Γ; tcrush. Qed.
 
 Example loopTyp Γ : Γ v⊢ₜ[∅] hclose hloopTm : ⊥.
 Proof.
-  have ? := loopFunTyp Γ; apply (iT_All_E (T1 := ⊤)), (iT_Sub_nocoerce 𝐍); tcrush.
+  have ? := loopFunTyp Γ; apply (iT_All_E (T1 := ⊤)), (iT_Sub_nocoerce 𝐙); tcrush.
 Qed.
 
 (** XXX Not currently using olty. *)
@@ -111,7 +111,7 @@ Section s_is_pos.
 Context `{HdlangG: dlangG Σ}.
 Context (s: stamp).
 
-Definition pos v := ∃ n, v = vnat n ∧ n > 0.
+Definition pos v := ∃ n, v = vint n ∧ n > 0.
 Definition ipos: oltyO Σ 0 := olty0 (λI ρ v, ⌜ pos v ⌝).
 
 Definition Hs := (s ↝n[ 0 ] ipos)%I.
@@ -157,7 +157,7 @@ Section div_example.
   Qed.
 
   Lemma wp_if_ge' (n : nat) :
-    WP tif (n > 0) (1 `div` n) (hclose hloopTm) {{ w, ⟦ 𝐍 ⟧ ids w ∧ ⌜ n > 0 ⌝}}%I.
+    WP tif (n > 0) (1 `div` n) (hclose hloopTm) {{ w, ⟦ 𝐙 ⟧ ids w ∧ ⌜ n > 0 ⌝}}%I.
   Proof using Type*.
     wp_bind (IfCtx _ _).
     wp_bin; ev; simplify_eq/=.
@@ -192,9 +192,9 @@ Section div_example.
   Import hoasNotation.
 
   Definition posModT := μ: self, {@
-    type "Pos" >: ⊥ <: 𝐍;
-    val "mkPos" : 𝐍 →: self @; "Pos";
-    val "div" : 𝐍 →: self @; "Pos" →: 𝐍
+    type "Pos" >: ⊥ <: 𝐙;
+    val "mkPos" : 𝐙 →: self @; "Pos";
+    val "div" : 𝐙 →: self @; "Pos" →: 𝐙
   }.
 
   Definition hdivV := λ: m n, (htskip m) `div` n.
@@ -211,16 +211,16 @@ Section div_example.
   Lemma sToIpos : Hs -∗ dtysem [] s ↗n[ 0 ] hoEnvD_inst [] ipos.
   Proof. by iApply dm_to_type_intro. Qed.
 
-  Lemma Sub_ipos_nat Γ : Γ s⊨ ipos, 0 <: V⟦ 𝐍 ⟧, 0.
+  Lemma Sub_ipos_nat Γ : Γ s⊨ ipos, 0 <: V⟦ 𝐙 ⟧, 0.
   Proof.
     rewrite /ipos /pos /= /pure_interp_prim /prim_evals_to /=.
     iIntros "!>" (ρ w) "_ % !%"; naive_solver.
   Qed.
 
-  Lemma Sub_later_ipos_nat Γ : Γ s⊨ oLater ipos, 0 <: oLater V⟦ 𝐍 ⟧, 0.
+  Lemma Sub_later_ipos_nat Γ : Γ s⊨ oLater ipos, 0 <: oLater V⟦ 𝐙 ⟧, 0.
   Proof. rewrite -sSub_Later_Sub -sSub_Index_Incr. apply Sub_ipos_nat. Qed.
 
-  Lemma sHasA' l Γ : Hs -∗ Γ s⊨ { l := dtysem [] s } : C⟦ type l >: ⊥ <: 𝐍 ⟧.
+  Lemma sHasA' l Γ : Hs -∗ Γ s⊨ { l := dtysem [] s } : C⟦ type l >: ⊥ <: 𝐙 ⟧.
   Proof.
     iIntros "Hs".
     iApply (sD_Typ_Abs ipos); [|iApply sBot_Sub|by iExists _; iFrame "Hs"].
@@ -233,20 +233,20 @@ Section div_example.
   Proof. constructor; naive_solver. Qed.
   Hint Resolve sInTestVl : core.
 
-  Lemma sHasA l : Hs -∗ D*⟦ type l >: ⊥ <: 𝐍 ⟧ ids (dtysem [] s).
+  Lemma sHasA l : Hs -∗ D*⟦ type l >: ⊥ <: 𝐙 ⟧ ids (dtysem [] s).
   Proof.
     rewrite (sHasA' l []); iIntros "H".
     by iDestruct ("H" $! (testVl l .: ids) with "[] []") as "[_ $]".
   Qed.
 
-  Lemma posModVHasAtyp: Hs -∗ [] ⊨ posModV : type "Pos" >: ⊥ <: TNat.
+  Lemma posModVHasAtyp: Hs -∗ [] ⊨ posModV : type "Pos" >: ⊥ <: TInt.
   Proof.
     rewrite -ietp_value; iIntros "#Hs" (ρ).
     iExists _; iSplit; by [eauto | iApply (sHasA "Pos")].
   Qed.
 
   Lemma ty_mkPos :
-    [] s⊨ hclose hmkPosV : oAll V⟦ 𝐍 ⟧ (olty0 (λI ρ v, ⌜ ∃ n : nat, v = n ∧ n > 0 ⌝)).
+    [] s⊨ hclose hmkPosV : oAll V⟦ 𝐙 ⟧ (olty0 (λI ρ v, ⌜ ∃ n : nat, v = n ∧ n > 0 ⌝)).
   Proof using Type*.
     rewrite -sT_All_I /= /shead.
     iIntros (ρ) "!> /=". iDestruct 1 as %(_ & n & Hw); simplify_eq/=; rewrite Hw.
@@ -254,10 +254,10 @@ Section div_example.
   Qed.
 
   Lemma wp_mkPos :
-    oAll V⟦ 𝐍 ⟧ (olty0 (λI ρ v, ⌜ ∃ n : nat, v = n ∧ n > 0 ⌝)) vnil ids (hclose hmkPosV).
+    oAll V⟦ 𝐙 ⟧ (olty0 (λI ρ v, ⌜ ∃ n : nat, v = n ∧ n > 0 ⌝)) vnil ids (hclose hmkPosV).
   Proof using Type*. iApply wp_value_inv'. iApply (ty_mkPos with "[//]"). Qed.
 
-  Lemma wp_div_spec (m : nat) w : ipos vnil ids w -∗ WP m `div` w {{ ⟦ 𝐍 ⟧ ids }}.
+  Lemma wp_div_spec (m : nat) w : ipos vnil ids w -∗ WP m `div` w {{ ⟦ 𝐙 ⟧ ids }}.
   Proof. iDestruct 1 as %(n&?&?); simplify_eq. wp_bin. by iIntros "!%"; naive_solver. Qed.
 
   Lemma posModVHasA: Hs -∗ [] ⊨ posModV : hclose posModT.
@@ -297,7 +297,7 @@ Section wp_inv.
     WP e {{ φ }} ⊢ ∃ e2, ⌜ prim_step e tt [] e2 tt [] ⌝ ∧ ▷ WP e2 {{ φ }}.
   Proof.
     rewrite wp_unfold/wp_pre/= {}Hne; iIntros "Hwp".
-    iDestruct ("Hwp" $! () [] [] 0 with "[//]") as (Hred) "Hwp".
+    iDestruct ("Hwp" $! () [] [] 0%nat with "[//]") as (Hred) "Hwp".
     destruct Hred as (? & e2 & [] & ? & Hr%prim_step_view).
     iDestruct ("Hwp" $! e2 with "[%//]") as "(_ & Heq & _)".
     by iExists _; iFrame.
@@ -336,27 +336,27 @@ Section small_ex.
 
   Definition v := ν {@
     type "A" = ([]; s);
-    val "n" = pv (vnat 2)
+    val "n" = pv (vint 2)
   }.
 
   Definition vTyp1Body : ty := {@
-    type "A" >: ⊥ <: 𝐍;
+    type "A" >: ⊥ <: 𝐙;
     val "n" : p0 @; "A"
   }.
   Definition vTyp1 := μ vTyp1Body.
 
 
   (** Yes, v has a valid type member. *)
-  Lemma vHasA0typ: Hs -∗ [] ⊨ tv v : type "A" >: ⊥ <: 𝐍.
+  Lemma vHasA0typ: Hs -∗ [] ⊨ tv v : type "A" >: ⊥ <: 𝐙.
   Proof.
     iIntros "#Hs".
-    iApply (T_Sub (i := 0) (T1 := μ {@ type "A" >: ⊥ <: 𝐍})).
+    iApply (T_Sub (i := 0) (T1 := μ {@ type "A" >: ⊥ <: 𝐙})).
     iApply T_Obj_I.
     iApply D_Cons; [done| by iApply sHasA'|].
     iSplit; [iIntros "!%"|iIntros "!> ** //"].
     repeat constructor; exact: not_elem_of_nil.
     iApply Sub_Trans.
-    iApply (Mu_Sub {@ type "A" >: ⊥ <: 𝐍}).
+    iApply (Mu_Sub {@ type "A" >: ⊥ <: 𝐙}).
     iApply sAnd1_Sub.
   Qed.
   (* This works. Crucially, we use T_Mu_I to introduce the object type.
@@ -377,7 +377,7 @@ Section small_ex.
     - iApply (T_Sub (i := 0) (T2 := TTop)); last by iApply sSub_Top.
       by iApply vHasA0typ.
     - rewrite -setp_value_eq /= /iPPred_car /=.
-      have Hev2: pos (vnat 2) by rewrite /pos; eauto.
+      have Hev2: pos (vint 2) by rewrite /pos; eauto.
       iIntros (_).
 
       repeat (repeat iExists _; repeat iSplit; rewrite ?path_wp_pv_eq //);
@@ -395,13 +395,13 @@ Section small_ex.
     see concretely below.
   *)
   Definition vTyp2Body : ty := {@
-    type "A" >: ⊥ <: 𝐍;
+    type "A" >: ⊥ <: 𝐙;
     val "n" : TLater (p0 @; "A")
   }.
   Definition vTyp2 := μ vTyp2Body.
 
   Definition svTyp2Body : oltyO Σ 0 :=
-    oAnd (cTMem "A" oBot (oPrim tnat))
+    oAnd (cTMem "A" oBot (oPrim tint))
       (oAnd (cVMem "n" (oLater (oSel p0 "A")))
       oTop).
   Goal V⟦vTyp2Body⟧ = svTyp2Body. done. Abort.
